pulse/lib/steel/pulse/Pulse.Checker.AssertWithBinders.fsti
@@ -6,13 +6,12 @@ open Pulse.Syntax
 open Pulse.Typing
 open Pulse.Checker.Common
 
+val check
+  (g:env)
+  (st:st_term { Tm_ProofHintWithBinders? st.term })
+  (pre:term)
+  (pre_typing:tot_typing g pre tm_vprop)
+  (post_hint:post_hint_opt g)
+  (check:check_t)
+  : T.Tac (checker_result_t g pre post_hint)
 
-// val check
-//   (g:env)
-//   (st:st_term{Tm_ProofHintWithBinders? st.term})
-//   (pre:term)
-//   (pre_typing:tot_typing g pre tm_vprop)
-//   (post_hint:post_hint_opt g)
-//   (frame_pre:bool)
-//   (check:check_t)
-//   : T.Tac (checker_result_t g pre post_hint frame_pre)
